cogent/examples/wa_connect/Generated_CorresProof.thy
@@ -76,10 +76,6 @@ ML \<open>
 fun typing_tree_of "wordarray_get_u32" = wordarray_get_u32_typing_tree
   | typing_tree_of "wordarray_length_u32" = wordarray_length_u32_typing_tree
   | typing_tree_of "wordarray_put2_u32" = wordarray_put2_u32_typing_tree
-  | typing_tree_of "dec" = dec_typing_tree
-  | typing_tree_of "dec_arr" = dec_arr_typing_tree
-  | typing_tree_of "inc" = inc_typing_tree
-  | typing_tree_of "inc_arr" = inc_arr_typing_tree
   | typing_tree_of "mul" = mul_typing_tree
   | typing_tree_of "mul_arr" = mul_arr_typing_tree
   | typing_tree_of "sum" = sum_typing_tree
@@ -149,10 +145,6 @@ val entry_func_names = [
       "wordarray_length_u32",
       "wordarray_get_u32",
       "wordarray_put2_u32",
-      "inc",
-      "dec",
-      "inc_arr",
-      "dec_arr",
       "sum",
       "mul",
       "sum_arr",
