cogent/isa/UpdateSemantics.thy
@@ -171,7 +171,7 @@ locale update_sem =
   and     abs_typing_readonly : "sigil_perm s \<noteq> Some Writable \<Longrightarrow> abs_typing av n \<tau>s s r w \<sigma> \<Longrightarrow> w = {}"
   and     abs_typing_escape   : "sigil_perm s \<noteq> Some ReadOnly \<Longrightarrow> [] \<turnstile>* \<tau>s :\<kappa> k \<Longrightarrow> E \<in> k \<Longrightarrow> abs_typing av n \<tau>s s r w \<sigma> \<Longrightarrow> r = {}"
   and     abs_typing_valid : "abs_typing av n \<tau>s s r w \<sigma> \<Longrightarrow> p \<in> r \<union> w \<Longrightarrow> \<sigma> p \<noteq> None"
-  and     abs_typing_unique_repr   : "abs_typing av n \<tau>s s r w \<sigma> \<Longrightarrow> abs_typing av n' \<tau>s' s' r' w' \<sigma>
+  and     abs_typing_unique_repr   : "abs_typing av n \<tau>s s r w \<sigma> \<Longrightarrow> abs_typing av n' \<tau>s' s' r' w' \<sigma>'
                                     \<Longrightarrow> type_repr (TCon n \<tau>s s) = type_repr (TCon n' \<tau>s' s')"
   and     abs_typing_repr : "abs_typing av n \<tau>s s r w \<sigma> \<Longrightarrow> abs_repr av = (n, map type_repr \<tau>s)"
   and     abs_typing_frame: "\<And> w1 w2 \<sigma>'. abs_typing av n \<tau>s s r w \<sigma> \<Longrightarrow> frame \<sigma> w1 \<sigma>' w2 \<Longrightarrow>
